WIP: proving cancel main

theories/cancellation/CancelMain.v
@@ -1,7 +1,7 @@
 Require Import CRIS.
 Require Import LMod LModTr GSim GSimFacts GSimTactics.
 Require Import MInline MInlineIntro MInlineElim.
-Require Import CancelCore CancelPG CancelAG CancelSpawn CancelPre CancelPost.
+Require Import ElimRel.
 
 Set Implicit Arguments.
 
@@ -43,18 +43,110 @@ Module CancelMain. Section CancelMain.
 
 Context `{_crisG: !crisG Γ Σ α β τ _S _I, _concG: !concG}.
 
+Lemma main_smod_find_some_eq md fn :
+  alist_find (Some fn) (MainSMod.map_fnsems (sp_from md) (SMod.fnsems md)) =
+    alist_find (Some fn) (map (map_snd (SModTr.trans_ktree (sp_from md))) (SMod.fnsems md)).
+Proof.
+  rewrite alist_find_map_snd MainSMod.alist_find_map_fnsems.
+  destruct (alist_find (Some fn) (SMod.fnsems md)); ss.
+Qed.
+
+Lemma main_smod_sandboxed_prog_eq md :
+  sandboxed_prog (MainSMod.to_mod (sp_from md) md) = sandboxed_prog (SMod.to_mod (sp_from md) md).
+Proof.
+  eapply func_ext. i.
+  rewrite /sandboxed_prog.
+  eapply func_ext. i.
+  rewrite main_smod_find_some_eq /SMod.to_mod /=. refl.
+Qed.
+
+Lemma main_smod_lmod_prog_eq md rs :
+  LMod.prog (Mod.to_lmod (MInline.inline (MainSMod.to_mod (sp_from md) md)) rs) =
+    LMod.prog (Mod.to_lmod (MInline.inline (SMod.to_mod (sp_from md) md)) rs).
+Proof.
+  eapply func_ext. i.
+  rewrite /LMod.prog /Mod.to_lmod /=.
+  rewrite !alist_find_map_snd MainSMod.alist_find_map_fnsems.
+  destruct (alist_find (Some x) (SMod.fnsems md)); ss.
+  rewrite /inline_fsem main_smod_sandboxed_prog_eq.
+  rewrite /MainSMod.trans_ktree; ss.
+Qed.
+
+
+Inductive cancel_main_inv md (cid: nat) (src tgt : list (itree lmodE Any.t)) :=
+| cancel_main_intro itr msk scp
+    (CID: cid < length src)
+    (LEN: length src = length tgt)
+    (SRC0: src !! 0 = Some itr)
+    (TGT0: tgt !! 0 =
+             Some
+               (st <- itr;;
+                ModTr.trans
+                  (inline_body (sandboxed_prog (SMod.to_mod (sp_from md) md))
+                     (interpV (SB.handle_sandbox true msk scp) (ret <- trigger (Choose Any.t);; trigger (Guarantee ⌜st = ret⌝);;; Ret ret)))))
+    (OTH: ∀ cid, cid <> 0 → src !! cid = tgt !! cid)
+  : cancel_main_inv md cid src tgt.
+
+Lemma cancel_main_aux md rs src tgt cid ps pt (INV: cancel_main_inv md cid src tgt)
+  (VALID: ✓ rs) :
+  gsim cancel_eq ps pt
+    (LModTr.interp_stateE Any.t
+       (iterV (LModTr.handle_callE (LMod.prog (Mod.to_lmod (MInline.inline (SMod.to_mod (sp_from md) md)) rs))) (cid, src))
+       (Any.pair (ModTr.alist_encode (SMod.initial_st md)) rs ↑))
+    (LModTr.interp_stateE Any.t
+       (iterV (LModTr.handle_callE (LMod.prog (Mod.to_lmod (MInline.inline (SMod.to_mod (sp_from md) md)) rs))) (cid, tgt))
+       (Any.pair (ModTr.alist_encode (SMod.initial_st md)) rs ↑)).
+Proof.
+  ginit. revert INV ps pt. revert cid src tgt. gcofix CIH; i.
+  destruct (decide (cid < length src)); cycle 1.
+  { dup n. inv INV. eapply not_lt in n. eapply lookup_ge_None in n.
+    ziter_l; rewrite n; zstep_l. }
+  destruct (decide (cid = 0)).
+  { subst. inv INV.
+    ides itr.
+    - ziter_r; rewrite TGT0 /=; zstep_r.
+      ziter_l; rewrite SRC0 /=; zstep_l.
+      zstep_r. ziter_r. zstep_r.
+      ziter_r. zstep_r. ired. ziter_r. zstep_r. zstep_r.
+      ziter_r. zstep_r. zstep_r. ziter_r. zstep_r.
+      ziter_r. zstep_r. ziter_r. zstep_r. ziter_r. zstep_r.
+      zstep. des.
+      assert (I: Own rs ⊢ ⌜r0 = x⌝).
+      { rewrite x2. iIntros ">[$ _]". }
+      eapply Own_pure_soundness in I; eauto; subst.
+      econs; esplits; eauto; rewrite Any.pair_split; ss.
+    - ziter_l; rewrite SRC0 /=; zstep_l.
+      ziter_r; rewrite TGT0 /=; zstep_r.
+      gstep. econs. econs; try exact smj_lt_mid_top.
+      gbase. eapply CIH. econs; eauto.
+      { rewrite length_insert //. }
+      { rewrite !length_insert //. }
+      { rewrite list_lookup_insert //. }
+      { rewrite list_lookup_insert // -LEN //. }
+      { i. rewrite !list_lookup_insert_ne //. eapply OTH; eauto. }
+    - admit.
+  }
+  eapply lookup_lt_is_Some in l. rewrite /is_Some in l. des.
+  inv INV. specialize (OTH cid). hexploit OTH; eauto; i.
+  ides x.
+  - ziter_l; rewrite l /=; zstep_l.
+    ziter_r; rewrite -H l /=; zstep_r. des_ifs. zstep_l.
+  - ziter_l; rewrite l /=; zstep_l.
+    ziter_r; rewrite -H l /=; zstep_r.
+Admitted.
+      
 Lemma cancel_main md rs
   (WFS: SMod.wf md)
   (WF: Mod.wf (SMod.to_mod sp_none (SMod.cancel md)))
   (VALID: ✓ rs)
   :  
   refines_lmod
-    (Mod.to_lmod (MInline.inline false (MainSMod.to_mod (sp_from md) md)) rs)
-    (Mod.to_lmod (MInline.inline false (SMod.to_mod (sp_from md) md)) rs).
+    (Mod.to_lmod (MInline.inline (MainSMod.to_mod (sp_from md) md)) rs)
+    (Mod.to_lmod (MInline.inline (SMod.to_mod (sp_from md) md)) rs).
 Proof using.
   r. intro arg. eapply gsim_adequacy.
   instantiate (1:= smj_top). instantiate (1:= smj_top).
-  unfold LMod.compile. s. rewrite /ITree.map /LModTr.trans /LModTr.interp_callE.  
+  unfold LMod.compile. s. rewrite /ITree.map /LModTr.trans /LModTr.interp_callE.
 
   rewrite !alist_find_map_snd.
   rewrite !MainSMod.alist_find_map_fnsems.
@@ -73,12 +165,35 @@ Proof using.
 
   r in WFS. hexploit WFS; eauto; i; des; ss.
   hexploit H1; eauto; i; subst; ss.
-
-  ziter_l. zstep_l. ziter_l. zstep_l.
-  exploit WFS; et. i; des; subst; ss.
   
-  ginit. guclo bindC_spec. econs; cycle 1.
-  { instantiate (1:=cancel_eq). i. gstep. econs. econs.
-    destruct SIM. des. et. }
   ziter_l. zstep_l. ziter_l. zstep_l.
   exploit WFS; et. i; des; subst; ss.
+
+  rewrite main_smod_sandboxed_prog_eq.
+  rewrite main_smod_lmod_prog_eq.
+  
+  ziter_r. zstep_r. exists tt. zstep_r.
+  ziter_r. zstep_r. ziter_r. zstep_r. exists arg. zstep_r.
+  ziter_r. zstep_r. ziter_r. zstep_r. ired.
+  ziter_r. zstep_r. exists rs. zstep_r.
+  ziter_r. zstep_r. unshelve eexists.
+  { split; eauto. }
+  zstep_r. ziter_r. zstep_r.
+  ziter_r. zstep_r. ziter_r. zstep_r.
+
+  set (temp:=interpV _ _) at 2.
+  set (itr:=_:itree crisE Any.t) in temp at 2.
+  replace temp with (SB.sandbox true msk scp itr); cycle 1.
+  { subst itr temp; refl. }
+  subst temp itr. rewrite SBRed.bind MIRed.bind Red.bind /SB.sandbox.
+
+  remember (ModTr.trans (inline_body (sandboxed_prog (SMod.to_mod (sp_from md) md)) (interpV (SB.handle_sandbox true msk scp) (SModTr.trans true (sp_from md) (bd arg))))) as itr.
+
+  gfinal. right.
+  eapply cancel_main_aux; eauto.
+  econs; eauto.
+  i. assert (LE: cid >= 1) by nia. dup LE.
+  replace 1 with (length [itr]) in LE by ss.
+  eapply lookup_ge_None in LE.
+
+Admitted.
